Printing.v
@@ -1,0 +1,64 @@
+From QuickChick Require Import QuickChick Tactics.
+Import QcNotation QcDefaultNotation. Open Scope qc_scope.
+Require Export ExtLib.Structures.Monads.
+Require Import ExtLib.Data.List.
+Import MonadNotation.
+
+From SECF Require Import MiniCET.
+
+Derive Show for observation.
+
+#[export] Instance showVal : Show val :=
+  {show :=fun v => 
+      match v with
+      | N n => show n
+      | FP l => ("&" ++ show l)%string
+      | UV => "UV"%string
+      end
+  }.
+  
+#[export] Instance showBinop : Show binop :=
+  {show :=fun op => 
+      match op with
+      | BinPlus => "+"%string
+      | BinMinus => "-"%string  
+      | BinMult => "*"%string
+      | BinEq => "="%string
+      | BinLe => "<="%string
+      | BinAnd => "&&"%string
+      | BinImpl => "->"%string
+      end
+  }.
+
+#[export] Instance showExp : Show exp :=
+  {show := 
+    (let fix showExpRec (e : exp) : string :=
+       match e with
+       | ANum n => show n
+       | AId x => x
+       | ABin o e1 e2 => 
+           "(" ++ showExpRec e1 ++ " " ++ show o ++ " " ++ showExpRec e2 ++ ")"
+       | ACTIf b e1 e2 =>
+           "(" ++ showExpRec b ++ " ? " ++ showExpRec e1 ++ " : " ++ showExpRec e2 ++ ")"
+       | FPtr l => "&" ++ show l
+       end
+     in showExpRec)%string
+  }.
+
+#[export] Instance showInst : Show inst :=
+  {show := 
+      (fun i =>
+         match i with
+         | ISkip => "skip"
+         | IAsgn x e => x ++ " := " ++ show e
+         | IBranch e l => "branch " ++ show e ++ " to " ++ show l
+         | IJump l => "jump " ++ show l
+         | ILoad x a => x ++ " <- load[" ++ show a ++ "]"
+         | IStore a e => "store[" ++ show a ++ "] <- " ++ show e
+         | ICall fp => "call " ++ show fp
+         | ICTarget => "ctarget"
+         | IRet => "ret"
+         end)%string
+  }.
+
+Derive Show for ty.
